\documentclass{article}
\usepackage{fullpage}
\usepackage{titlesec}
\usepackage{graphicx}
\usepackage{amsmath}
\usepackage{amssymb}
\usepackage{verbatim}

% Definition of \subparagraph starting new line after heading
\titleformat{\subparagraph}
    {\normalfont\normalsize\bfseries}{\thesubparagraph}{1em}{}
\titlespacing*{\subparagraph}{\parindent}{3.25ex plus 1ex minus .2ex}{.75ex plus .1ex}
\titleformat{\paragraph}
    {\normalfont\normalsize\bfseries}{\theparagraph}{1em}{}
\titlespacing*{\paragraph}{\parindent}{3.25ex plus 1ex minus .2ex}{.75ex plus .1ex}

\begin{document}


\begin{flushright}
Jeffrey Whissen
\\MTH 256 DiffEq.
\\Homework \#8
\\Due: 8/16/2012
\end{flushright}

5.1: (20, 22, 24);
6.1: (16, 18, 20);
6.2: (8, 10, 12);
6.3: (28, 30, 32)\\




\paragraph{Chapter 6.3}

\subparagraph{28.}
\begin{tabular}{ r  p{10cm} }
a & \\
 &$\mathcal{L}[\frac{d^2y}{dt^2}] - \mathcal{L}[y] = \mathcal{L}[e^{2t}] $\\
 &$s^2\mathcal{L}[y] - sy(0) - y`(0) - \mathcal{L}[y] = \frac{1}{s-2}$\\
 &$(s^2 - 1)\mathcal{L}[y] - sy(0) - y`(0) = \frac{1}{s-2}$\\
b & \\
 &$(s^2 - 1)\mathcal{L}[y] - s + 1 = \frac{1}{s-2}$\\
 &$\mathcal{L}[y]= \frac{1}{(s-2)(s^2 - 1)} + \frac{s}{s^2 - 1} - \frac{1}{s^2 - 1}$\\
 &$\mathcal{L}[y]= \frac{1}{(s-2)(s^2 - 1)} + \frac{s}{s^2 - 1} - \frac{1}{s^2 - 1}$\\
 &$\mathcal{L}[y]= \frac{1}{(s-2)(s+1)(s-1)} + \frac{s}{(s+1)(s-1)} - \frac{1}{(s+1)(s-1)}$\\
 &$\mathcal{L}[y]= \frac{1}{(s-2)(s+1)(s-1)} + \frac{s - 1}{(s+1)(s-1)}$\\
 &$\mathcal{L}[y]= \frac{1}{(s-2)(s+1)(s-1)} + \frac{1}{(s+1)}$\\
 &$\mathcal{L}[y] = \frac{A}{s-2} + \frac{B}{s-1} + \frac{C}{s+1} + \frac{1}{(s+1)}$\\
 \\
 &Where: $A(s^2 - 1) + B(s^2-s-2) + C(s^2-3s+2) = 1$\\
 & $s^2(A+B+C) + s(-B-3C) - A - 2B + 2C  = 1$\\
 &$B=-3C; s^2(A-2C) - A + 8C  = 1$\\
 & $A=2C;  - 2C + 8C  = 1$\\
 & $C = \frac{1}{6}$\\
 \\
 &$\mathcal{L}[y] = \frac{1}{3}\frac{1}{s-2} - \frac{1}{2}\frac{1}{s-1} + \frac{1}{6}\frac{1}{s+1} + \frac{1}{(s+1)}$\\
 &$\mathcal{L}[y] = \frac{1}{3}\frac{1}{s-2} - \frac{1}{2}\frac{1}{s-1} + \frac{7}{6}\frac{1}{s+1}$\\
c & \\
 &$\mathcal{L}^{-1}[\mathcal{L}[y]] = \mathcal{L}^{-1}[\frac{1}{3}\frac{1}{s-2}] - \mathcal{L}^{-1}[\frac{1}{2}\frac{1}{s-1}] + \mathcal{L}^{-1}[\frac{7}{6}\frac{1}{s+1}]$\\
 &$y(t) = \frac{1}{3}e^{2t} - \frac{1}{2}e^{t} + \frac{7}{6}e^{-t}$\\
 \end{tabular}

  
\end{tabular}



\end{document}

